Kraken/Examples/SimplifiedSemanticsExample.lean
@@ -1,0 +1,42 @@
+import Kraken.Tactics
+import Kraken.Parser
+import Kraken.Eval
+import Kraken.SimplifiedSemantics
+
+open Kraken.Parser
+
+-- This is the same as p2 in Examples, but without using Executable
+def p2 : List Directive := [
+  .label "start",
+  .instr ⟨ .W64, .W64, .mov Reg.rax (.imm (.int64 1)) ⟩,
+  .instr ⟨ .W64, .W64, .xor Reg.rax Reg.rax ⟩,
+  .instr ⟨ .W64, .W64, .jcc .nz "start" ⟩,
+  .instr ⟨ .W64, .W64, .mov Reg.rax (.imm (.int64 2)) ⟩,
+]
+
+-- Replicate the example using the simplified transition relation and polymorphic Eventually
+example (s : MachineData) :
+  Eventually (simplified_step1 p2) (fun s' => s'.1.regs.rax = 2) (s, Int64.ofNat 0) := by
+  dsimp [p2]
+
+  -- initial label
+  apply step_cps
+  dsimp only [simplified_step1,Kraken.Simplified.step]
+  simp -- At this point we have simplified the match term from Simplified.step
+  dsimp only [Directive.interp, Effects.all]
+
+  -- first mov
+  apply step_cps
+  dsimp only [simplified_step1, Kraken.Simplified.step]
+  simp -- following line does symbolic execution
+  dsimp only [Directives.interp,Directive.interp,Instr.interp,Operation.interp,Operand.interp,RegOrMem.interp]
+  dsimp only [MachineData.set,Reg64s.set,MachineData.setReg,Reg64s.set64,ConstExpr.interp,CondCode.interp,StatusFlags.from_result, Effects.all]
+
+  -- second step: xor %rax, %rax
+  apply step_cps
+  dsimp only [simplified_step1, Kraken.Simplified.step]
+  simp
+  dsimp only [Directives.interp,Directive.interp,Instr.interp,Operation.interp,Operand.interp,RegOrMem.interp]
+  dsimp only [MachineData.set,Reg64s.set,MachineData.setReg,Reg64s.set64,ConstExpr.interp,CondCode.interp,StatusFlags.from_result, Effects.all]
+
+  sorry
